
\documentclass[fleqn]{exam}
\usepackage{amsmath,amsthm,amssymb}
\usepackage{multicol}
\usepackage{enumitem}
\rhead{Robert Smith}
\lhead{John Jerk - Lesson 4 Homework}
\begin{document}

\section{Algebra}

\begin{multicols}{2}
\begin{enumerate}[label=(\alph*)]
\item $ \displaystyle \frac{x}{z} + 5 = x z\\x = \frac{5 z}{z^{2} - 1}$
\item $ \displaystyle \frac{x}{100} = x + 6\\x = - \frac{200}{33}$
\item $ \displaystyle z \left(x - z\right) = x - z\\x = z$
\item $ \displaystyle x + 10 = 3 x\\x = 5$
\item $ \displaystyle \frac{x}{8} + 1 = x - z\\x = \frac{8 z}{7} + \frac{8}{7}$
\item $ \displaystyle \frac{x}{z} + z = x - 1\\x = \frac{z \left(z + 1\right)}{z - 1}$
\item $ \displaystyle \frac{x}{3} - z = x - 7\\x = - \frac{3 z}{2} + \frac{21}{2}$
\item $ \displaystyle x + 2 z = x z\\x = \frac{2 z}{z - 1}$
\item $ \displaystyle \frac{x}{2} - y = 2 x\\x = - \frac{2 y}{3}$
\item $ \displaystyle x - z + 3 = 2 x\\x = - z + 3$
\item $ \displaystyle 10 x + 1 = 6 x\\x = - \frac{1}{4}$
\item $ \displaystyle 2 x + 4 = x + 1\\x = -3$
\item $ \displaystyle \frac{x}{2} - 2 = x + z\\x = - 2 z - 4$
\item $ \displaystyle x + y + 8 = 2 x\\x = y + 8$
\item $ \displaystyle 2 x - 1 = x + 5\\x = 6$

\end{enumerate}
\end{multicols}

\newpage
\section*{Answers}

\section{Algebra}

\begin{multicols}{2}
\begin{enumerate}[label=(\alph*)]
\item $ \displaystyle x = \frac{5 z}{z^{2} - 1}$
\item $ \displaystyle x = - \frac{200}{33}$
\item $ \displaystyle x = z$
\item $ \displaystyle x = 5$
\item $ \displaystyle x = \frac{8 z}{7} + \frac{8}{7}$
\item $ \displaystyle x = \frac{z \left(z + 1\right)}{z - 1}$
\item $ \displaystyle x = - \frac{3 z}{2} + \frac{21}{2}$
\item $ \displaystyle x = \frac{2 z}{z - 1}$
\item $ \displaystyle x = - \frac{2 y}{3}$
\item $ \displaystyle x = - z + 3$
\item $ \displaystyle x = - \frac{1}{4}$
\item $ \displaystyle x = -3$
\item $ \displaystyle x = - 2 z - 4$
\item $ \displaystyle x = y + 8$
\item $ \displaystyle x = 6$

\end{enumerate}
\end{multicols}

\end{document}
