
\documentclass[fleqn]{exam}
\usepackage{amsmath,amsthm,amssymb}
\usepackage{multicol}
\usepackage{enumitem}
\rhead{Robert Smith}
\lhead{Jackson Serratore - Lesson 13 Homework}
\begin{document}

\section{Algebra}

\begin{multicols}{2}
\begin{enumerate}[label=(\alph*)]
\item $ \displaystyle \frac{x}{7} = 6 y$
\item $ \displaystyle 7 y + \frac{x z}{2} = 3$
\item $ \displaystyle \frac{\frac{1}{6} x}{8} + 7 y = 2$
\item $ \displaystyle 2 y + \frac{7}{x \frac{1}{z}} = 4 y$
\item $ \displaystyle y + \frac{6}{x + 3} = 5 y$
\item $ \displaystyle 9 y + \frac{1}{x + y} = 2 y$

\end{enumerate}
\end{multicols}

\section{Fractions}

\begin{multicols}{2}
\begin{enumerate}[label=(\alph*)]
\item $ \displaystyle \frac{x}{7} + \frac{2}{7} = x + y$

\end{enumerate}
\end{multicols}

\newpage
\section*{Answers}

\section{Algebra}

\begin{multicols}{2}
\begin{enumerate}[label=(\alph*)]
\item $ \displaystyle x = 42 y$
\item $ \displaystyle x = \frac{2}{z} \left(- 7 y + 3\right)$
\item $ \displaystyle x = - 336 y + 96$
\item $ \displaystyle x = \frac{7 z}{2 y}$
\item $ \displaystyle x = -3 + \frac{3}{2 y}$
\item $ \displaystyle x = - y - \frac{1}{7 y}$

\end{enumerate}
\end{multicols}

\section{Fractions}

\begin{multicols}{2}
\begin{enumerate}[label=(\alph*)]
\item $ \displaystyle x = - \frac{7 y}{6} + \frac{1}{3}$

\end{enumerate}
\end{multicols}

\end{document}
